proof/uni/prop_basic.v
@@ -49,7 +49,7 @@ Qed.
 Lemma subst_typ_in_exp_open_exp_wrt_exp_fresh2: forall X e1 e2 A,
   lc_typ A ->
   X `notin` ftvar_in_exp e2 ->
-  (subst_typ_in_exp A X e1) ᵉ^ₑ e2 = subst_typ_in_exp A X (e1 ᵉ^ₑ e2).
+  (subst_typ_in_exp A X e1) ᵉ^^ₑ e2 = subst_typ_in_exp A X (e1 ᵉ^^ₑ e2).
 Proof.
   intros. 
   rewrite subst_typ_in_exp_open_exp_wrt_exp; auto.
@@ -60,7 +60,7 @@ Qed.
 Lemma subst_typ_in_exp_open_exp_wrt_typ_fresh2: forall X e A B,
   lc_typ A ->
   X `notin` ftvar_in_typ B ->
-  (subst_typ_in_exp A X e) ᵉ^ₜ B = subst_typ_in_exp A X (e ᵉ^ₜ B).
+  (subst_typ_in_exp A X e) ᵉ^^ₜ B = subst_typ_in_exp A X (e ᵉ^^ₜ B).
 Proof.
   intros. 
   rewrite subst_typ_in_exp_open_exp_wrt_typ; auto.
@@ -185,11 +185,34 @@ Proof.
     contradiction.
 Qed.
 
+Lemma subst_typ_in_exp_open_exp_wrt_typ_tvar2 : forall X e A,
+  lc_typ A ->
+  X `notin` ftvar_in_exp e ->
+  {A ᵉ/ₜ X} (e ᵉ^^ₜ ` X) = e ᵉ^^ₜ A.
+Proof.
+  intros.
+  rewrite subst_typ_in_exp_open_exp_wrt_typ; auto.
+  rewrite (subst_typ_in_exp_fresh_eq e); auto.
+  simpl. destruct_eq_atom; auto.
+Qed.
+
+
+Lemma subst_exp_in_exp_open_exp_wrt_exp_var2 : forall x e1 e2,
+  lc_exp e2 ->
+  x `notin` fvar_in_exp e1 ->
+  {e2 ᵉ/ₑ x} (e1 ᵉ^^ₑ (exp_var_f x)) = e1 ᵉ^^ₑ e2.
+Proof.
+  intros.
+  rewrite subst_exp_in_exp_open_exp_wrt_exp; auto.
+  rewrite (subst_exp_in_exp_fresh_eq e1); auto.
+  simpl. destruct_eq_atom; auto.
+Qed.
+
 
 Lemma open_typ_wrt_typ_twice : forall n X Y A,
-    lc_typ Y ->
-    open_typ_wrt_typ_rec n ` X (open_typ_wrt_typ_rec (n+1) Y A)
-    = open_typ_wrt_typ_rec n Y (open_typ_wrt_typ_rec n ` X A).
+  lc_typ Y ->
+  open_typ_wrt_typ_rec n ` X (open_typ_wrt_typ_rec (n+1) Y A) = 
+    open_typ_wrt_typ_rec n Y (open_typ_wrt_typ_rec n ` X A).
 Proof with subst; simpl in *; eauto; try lia.
   introv HL. gen n. induction A; intros...
   all: try congruence.
@@ -210,14 +233,13 @@ Proof with subst; simpl in *; eauto; try lia.
 Qed.
 
 
-
-Lemma typ_open_r_close_l : forall T1 T2 X, 
-  X `notin` ftvar_in_typ T2 -> 
-  T1 = open_typ_wrt_typ T2 ` X -> 
-  close_typ_wrt_typ X T1 = T2.
+Lemma typ_open_r_close_l : forall A B X, 
+  X `notin` ftvar_in_typ B -> 
+  A = open_typ_wrt_typ B ` X -> 
+  close_typ_wrt_typ X A = B.
 Proof.
   intros * Fr H.
-  assert (close_typ_wrt_typ X T1 = close_typ_wrt_typ X (open_typ_wrt_typ T2 ` X)) by now rewrite H.
+  assert (close_typ_wrt_typ X A = close_typ_wrt_typ X (open_typ_wrt_typ B ` X)) by now rewrite H.
   now rewrite close_typ_wrt_typ_open_typ_wrt_typ in H0.
 Qed.
 
@@ -345,7 +367,7 @@ Proof with eauto using lc_typ_subst.
   intros. induction H; simpl...
   - destruct_eq_atom; auto.
   - pick fresh x0. apply lc_exp_abs_exists with (x1:=x0). 
-    replace (({e2 ᵉ/ₑ x} e) ᵉ^ₑ exp_var_f x0) with ({e2 ᵉ/ₑ x} (e ᵉ^ₑ exp_var_f x0))...
+    replace (({e2 ᵉ/ₑ x} e) ᵉ^^ₑ exp_var_f x0) with ({e2 ᵉ/ₑ x} (e ᵉ^^ₑ exp_var_f x0))...
     rewrite subst_exp_in_exp_open_exp_wrt_exp... simpl; destruct_eq_atom...
   - pick fresh X0. apply lc_exp_tabs_exists with (X1:=X0).
     rewrite <- subst_exp_in_exp_open_exp_wrt_typ...
@@ -357,30 +379,30 @@ Lemma lc_exp_subst_typ_in_exp_inv : forall e A X,
   lc_typ A ->
   lc_exp e.
 Proof.
-  - intros. dependent induction H; auto; try solve [destruct e; try solve [inversion x]; auto].
-    + destruct e; try solve [inversion x]; auto.
-      inversion x. subst.
-      inst_cofinites_by (singleton X) using_name x.
-      apply lc_exp_abs_exists with (x1:=x0).
-      eapply H0 with (x:=x0) (X:=X); eauto.
-      rewrite subst_typ_in_exp_open_exp_wrt_exp; simpl; auto.
-    + destruct e; try solve [inversion x]; auto.
-      inversion x. subst.
-      constructor; eauto.
-    + destruct e; try solve [inversion x]; auto.
-      inversion x. subst.
-      inst_cofinites_by (singleton X) using_name X.
-      apply lc_exp_tabs_exists with (X1:=X0).
-      eapply H0; eauto.
-      rewrite subst_typ_in_exp_open_exp_wrt_typ_fresh2; eauto.
-    + destruct e; try solve [inversion x]; auto.
-      inversion x. subst.
-      constructor; eauto. 
-      eapply lc_typ_subst_inv; eauto.
-    + destruct e; try solve [inversion x]; auto.
-      inversion x. subst.
-      constructor; eauto.
-      eapply lc_typ_subst_inv; eauto.
+  intros. dependent induction H; auto; try solve [destruct e; try solve [inversion x]; auto].
+  - destruct e; try solve [inversion x]; auto.
+    inversion x. subst.
+    inst_cofinites_by (singleton X) using_name x.
+    apply lc_exp_abs_exists with (x1:=x0).
+    eapply H0 with (x:=x0) (X:=X); eauto.
+    rewrite subst_typ_in_exp_open_exp_wrt_exp; simpl; auto.
+  - destruct e; try solve [inversion x]; auto.
+    inversion x. subst.
+    constructor; eauto.
+  - destruct e; try solve [inversion x]; auto.
+    inversion x. subst.
+    inst_cofinites_by (singleton X) using_name X.
+    apply lc_exp_tabs_exists with (X1:=X0).
+    eapply H0; eauto.
+    rewrite subst_typ_in_exp_open_exp_wrt_typ_fresh2; eauto.
+  - destruct e; try solve [inversion x]; auto.
+    inversion x. subst.
+    constructor; eauto. 
+    eapply lc_typ_subst_inv; eauto.
+  - destruct e; try solve [inversion x]; auto.
+    inversion x. subst.
+    constructor; eauto.
+    eapply lc_typ_subst_inv; eauto.
 Qed.
 
 
