proof/uni_counter/algo_worklist/prop_soundness.v
@@ -1163,7 +1163,7 @@ Proof with eauto.
   - destruct_a_wf_wl.
     remember (fvar_in_exp e).
     pick fresh x. 
-    assert (⊢ᵃʷₛ (work_check (e ᵉ^ₑ exp_var_f x) A2 ⫤ᵃ x ~ᵃ A1;ᵃ Γ)). {
+    assert (⊢ᵃʷₛ (work_check (e ᵉ^^ₑ exp_var_f x) A2 ⫤ᵃ x ~ᵃ A1;ᵃ Γ)). {
       repeat (constructor; simpl; auto).
       eapply a_wf_exp_var_binds_another_cons...
       apply a_wf_typ_weaken_cons...
@@ -1191,11 +1191,11 @@ Proof with eauto.
     pick fresh x. pick fresh X1. pick fresh X2.
     inst_cofinites_with x. inst_cofinites_with X1. inst_cofinites_with X2.  
     assert (Hws: exists Γ1 Γ2, aworklist_subst 
-       (work_check (e ᵉ^ₑ exp_var_f x) ` X2  ⫤ᵃ x ~ᵃ ` X1;ᵃ X2 ~ᵃ ⬒ ;ᵃ X1 ~ᵃ ⬒ ;ᵃ Γ) X
+       (work_check (e ᵉ^^ₑ exp_var_f x) ` X2  ⫤ᵃ x ~ᵃ ` X1;ᵃ X2 ~ᵃ ⬒ ;ᵃ X1 ~ᵃ ⬒ ;ᵃ Γ) X
        (typ_arrow ` X1 ` X2) Γ1 Γ2). {
        eapply worklist_subst_fresh_etvar_total' with (X1:=X1) (X2:=X2) in H4 as Hws; auto.
        destruct Hws as [Γ1 [Γ2 Hws]].
-       exists Γ1, (work_check (e ᵉ^ₑ exp_var_f x) ` X2  ⫤ᵃ x ~ᵃ ` X1 ;ᵃ Γ2)...
+       exists Γ1, (work_check (e ᵉ^^ₑ exp_var_f x) ` X2  ⫤ᵃ x ~ᵃ ` X1 ;ᵃ Γ2)...
     }
     destruct Hws as [Γ1 [Γ2 Hsubst]].
     apply H6 in Hsubst as Hwsred.
@@ -1231,7 +1231,7 @@ Proof with eauto.
       * simpl. constructor... 
       * simpl...  
     + eapply aworklist_subst_wf_wl with 
-        (Γ:=(work_check (e ᵉ^ₑ exp_var_f x) ` X2  ⫤ᵃ x ~ᵃ ` X1;ᵃ X2 ~ᵃ ⬒ ;ᵃ X1 ~ᵃ ⬒ ;ᵃ Γ)); eauto. 
+        (Γ:=(work_check (e ᵉ^^ₑ exp_var_f x) ` X2  ⫤ᵃ x ~ᵃ ` X1;ᵃ X2 ~ᵃ ⬒ ;ᵃ X1 ~ᵃ ⬒ ;ᵃ Γ)); eauto. 
       * repeat (constructor; simpl; auto).
         apply a_wf_exp_var_binds_another_cons with (A1:=T)...
         rewrite_env ((x ~ abind_var_typ T) ++ ((X2, ⬒) :: (X1 ~ ⬒)) ++ ⌊ Γ ⌋ᵃ).
@@ -1239,7 +1239,7 @@ Proof with eauto.
       * simpl... constructor...
   (* \ x. e <= ⊤ *)
   - destruct_a_wf_wl. pick fresh x. inst_cofinites_with x. 
-    assert ( ⊢ᵃʷₛ (work_check (e ᵉ^ₑ exp_var_f x) typ_top ⫤ᵃ x ~ᵃ typ_bot;ᵃ Γ)). 
+    assert ( ⊢ᵃʷₛ (work_check (e ᵉ^^ₑ exp_var_f x) typ_top ⫤ᵃ x ~ᵃ typ_bot;ᵃ Γ)). 
     { repeat (constructor; simpl; auto). 
       eapply a_wf_exp_var_binds_another_cons; eauto.
     }
@@ -1284,7 +1284,7 @@ Proof with eauto.
   (* /\ a. e : A => _ *)
   - destruct_a_wf_wl. 
     pick fresh X. inst_cofinites_with X.
-    assert (Hwf: ⊢ᵃʷₛ (work_check (e ᵉ^ₜ ` X) (A ᵗ^ₜ X) ⫤ᵃ X ~ᵃ □ ;ᵃ work_applys cs (typ_all A) ⫤ᵃ Γ)). {
+    assert (Hwf: ⊢ᵃʷₛ (work_check (e ᵉ^^ₜ ` X) (A ᵗ^ₜ X) ⫤ᵃ X ~ᵃ □ ;ᵃ work_applys cs (typ_all A) ⫤ᵃ Γ)). {
       rewrite open_body_wrt_typ_anno in *.
       dependent destruction H0...
       dependent destruction H...
@@ -1340,7 +1340,7 @@ Proof with eauto.
   - destruct_a_wf_wl.
     pick fresh x. pick fresh X1. pick fresh X2.
     inst_cofinites_with x. inst_cofinites_with X1. inst_cofinites_with X2.
-    assert (Hwf: ⊢ᵃʷₛ (work_check (e ᵉ^ₑ exp_var_f x) ` X2  ⫤ᵃ x ~ᵃ ` X1;ᵃ work_applys cs (typ_arrow ` X1 ` X2)
+    assert (Hwf: ⊢ᵃʷₛ (work_check (e ᵉ^^ₑ exp_var_f x) ` X2  ⫤ᵃ x ~ᵃ ` X1;ᵃ work_applys cs (typ_arrow ` X1 ` X2)
             ⫤ᵃ X2 ~ᵃ ⬒ ;ᵃ X1 ~ᵃ ⬒ ;ᵃ Γ)). {
       repeat (constructor; simpl; auto).
       apply a_wf_exp_var_binds_another_cons with (A1:=T)...
